<?xml version="1.0"?>


<!DOCTYPE rdf:RDF [
    <!ENTITY ao "http://purl.org/ao/" >
    <!ENTITY dcterms "http://purl.org/dc/terms/" >
    <!ENTITY prov "http://www.w3.org/ns/prov#" >
    <!ENTITY foaf "http://xmlns.com/foaf/0.1/" >
    <!ENTITY ro "http://purl.org/wf4ever/ro#" >
    <!ENTITY roevo "http://purl.org/wf4ever/roevo#" >
    <!ENTITY owl "http://www.w3.org/2002/07/owl#" >
    <!ENTITY xsd "http://www.w3.org/2001/XMLSchema#" >
    <!ENTITY rdfs "http://www.w3.org/2000/01/rdf-schema#" >
    <!ENTITY terms "http://www.openarchives.org/ore/terms/" >
    <!ENTITY rdf "http://www.w3.org/1999/02/22-rdf-syntax-ns#" >
    <!ENTITY dc "http://purl.org/dc/elements/1.1/" >
]>


<rdf:RDF xmlns="http://www.semanticweb.org/owl/owlapi/turtle#"
     xml:base="http://www.semanticweb.org/owl/owlapi/turtle"
     xmlns:dc="http://purl.org/dc/elements/1.1/"
     xmlns:ro="http://purl.org/wf4ever/ro#"
     xmlns:prov="http://www.w3.org/ns/prov#"
     xmlns:foaf="http://xmlns.com/foaf/0.1/"
     xmlns:terms="http://www.openarchives.org/ore/terms/"
     xmlns:dcterms="http://purl.org/dc/terms/"
     xmlns:rdfs="http://www.w3.org/2000/01/rdf-schema#"
     xmlns:ao="http://purl.org/ao/"
     xmlns:roevo="http://purl.org/wf4ever/roevo#"
     xmlns:owl="http://www.w3.org/2002/07/owl#"
     xmlns:xsd="http://www.w3.org/2001/XMLSchema#"
     xmlns:rdf="http://www.w3.org/1999/02/22-rdf-syntax-ns#">
    <owl:Ontology rdf:about="http://purl.org/wf4ever/roevo">
        <rdfs:comment xml:lang="en">The Research Object Evolution Ontology (roevo) extends the ro ontology to capture the lifecycle and versioning of research objects. ro ontology and other extensions are described at http://wf4ever.github.io/ro/.
        roevo is also an extension of PROV ontology for describing Research Object evolution provenance. PROV ontology is described at http://www.w3.org/TR/prov-o/.</rdfs:comment>
        <owl:versionIRI rdf:resource="http://purl.org/wf4ever/roevo/0.6.1"/>
        <owl:versionInfo rdf:datatype="&xsd;string">0.6.1</owl:versionInfo>
        <dc:date rdf:datatype="&xsd;string">2014-01-15</dc:date>
        <dc:creator rdf:datatype="&xsd;string">Raul Palma</dc:creator>
        <dc:title rdf:datatype="&xsd;string">Research Object Evolution Ontology</dc:title>
        <dc:description rdf:datatype="&xsd;string">The Research Object Evolution Ontology (roevo) extends the ro ontology to capture the lifecycle and versioning of research objects (ROs). roevo is also an extension of PROV ontology for describing Research Object evolution provenance.
        roevo enables the representation of the different stages of the ROs lifecycle, their dependencies, as well as the corresponding versions of ROs and their aggregated resources, with the associated changes in these resources. 
        roevo follows a modular approach, enabling the creation of extensions for modeling detailed taxonomies of changes for particular resources, e.g., workflows.
        Additional information about roevo and background information is available at http://www.wf4ever-project.org/wiki/display/docs/RO+evolution</dc:description>
        <dc:description rdf:resource="http://www.wf4ever-project.org/wiki/download/attachments/2065027/ROevo_v0.4%2823%29.png"/>
        <dc:contributor rdf:datatype="&xsd;string">Jun Zhao</dc:contributor>
        <dc:contributor rdf:datatype="&xsd;string">Khalid Belhajjame</dc:contributor>
        <dc:contributor rdf:datatype="&xsd;string">Stian Soiland-Reyes</dc:contributor>
        <dc:contributor rdf:datatype="&xsd;string">Oscar Corcho</dc:contributor>
        <dc:rights rdf:datatype="&xsd;string">This ontology is distributed under Creative Commons Attribution 3.0 License - http://creativecommons.org/licenses/by/3.0</dc:rights>
    </owl:Ontology>
    


    <!-- 
    ///////////////////////////////////////////////////////////////////////////////////////
    //
    // Object Properties
    //
    ///////////////////////////////////////////////////////////////////////////////////////
     -->

    


    <!-- http://purl.org/ao/annotatesResource -->

    <owl:ObjectProperty rdf:about="&ao;annotatesResource"/>
    


    <!-- http://purl.org/wf4ever/roevo#fromVersion -->

    <owl:ObjectProperty rdf:about="&roevo;fromVersion">
        <rdfs:label>fromVersion</rdfs:label>
        <rdfs:comment>Associates the set of changes (roevo:ChangeSpecification) that were used (applied) by the pointed version of the resource (roevo:VersionableResource)</rdfs:comment>
        <rdfs:domain rdf:resource="&roevo;ChangeSpecification"/>
        <rdfs:range rdf:resource="&roevo;VersionableResource"/>
        <rdfs:subPropertyOf rdf:resource="&prov;used"/>
    </owl:ObjectProperty>
    


    <!-- http://purl.org/wf4ever/roevo#hasArchive -->

    <owl:ObjectProperty rdf:about="&roevo;hasArchive">
        <rdfs:label>hasArchive</rdfs:label>
        <rdfs:comment>Link a roevo:LiveRO with its archived version (roevo:ArchivedRO)</rdfs:comment>
        <rdfs:range rdf:resource="&roevo;ArchivedRO"/>
        <rdfs:domain rdf:resource="&roevo;LiveRO"/>
        <owl:inverseOf rdf:resource="&roevo;isArchiveOf"/>
    </owl:ObjectProperty>
    


    <!-- http://purl.org/wf4ever/roevo#hasChange -->

    <owl:ObjectProperty rdf:about="&roevo;hasChange">
        <rdfs:label>hasChange</rdfs:label>
        <rdfs:comment>Associates a roevo:Change to the roevo:ChangeSpecification including this change (in the set of changes generating a version of a resource)</rdfs:comment>
        <rdfs:range rdf:resource="&roevo;Change"/>
        <rdfs:domain rdf:resource="&roevo;ChangeSpecification"/>
    </owl:ObjectProperty>
    


    <!-- http://purl.org/wf4ever/roevo#hasPreviousChange -->

    <owl:ObjectProperty rdf:about="&roevo;hasPreviousChange">
        <rdfs:label>hasPreviousChange</rdfs:label>
        <rdfs:comment>Associates two roevo:Changes that occurred one after the other</rdfs:comment>
        <rdfs:range rdf:resource="&roevo;Change"/>
        <rdfs:domain rdf:resource="&roevo;Change"/>
    </owl:ObjectProperty>
    


    <!-- http://purl.org/wf4ever/roevo#hasRevision -->

    <owl:ObjectProperty rdf:about="&roevo;hasRevision">
        <rdfs:label>hasRevision</rdfs:label>
        <rdfs:comment>Inverse of prov:wasRevisionOf, where a revision is a derivation for which the resulting entity is a revised version of some original. Hence, it associates an entity with another entity derived from the former.</rdfs:comment>
        <owl:inverseOf rdf:resource="&prov;wasRevisionOf"/>
    </owl:ObjectProperty>
    


    <!-- http://purl.org/wf4ever/roevo#hasSnapshot -->

    <owl:ObjectProperty rdf:about="&roevo;hasSnapshot">
        <rdfs:label>hasSnapshot</rdfs:label>
        <rdfs:comment>Link a roevo:LiveRO with its different snapshots (roevo:SnapshotRO)</rdfs:comment>
        <rdfs:domain rdf:resource="&roevo;LiveRO"/>
        <rdfs:range rdf:resource="&roevo;SnapshotRO"/>
        <owl:inverseOf rdf:resource="&roevo;isSnapshotOf"/>
    </owl:ObjectProperty>
    


    <!-- http://purl.org/wf4ever/roevo#isArchiveOf -->

    <owl:ObjectProperty rdf:about="&roevo;isArchiveOf">
        <rdfs:label>isArchiveOf</rdfs:label>
        <rdfs:comment>Inverse of roevo:hasArchive. It associates an roevo:ArchivedRO with the roevo:LiveRO from which it was created</rdfs:comment>
    </owl:ObjectProperty>
    


    <!-- http://purl.org/wf4ever/roevo#isSnapshotOf -->

    <owl:ObjectProperty rdf:about="&roevo;isSnapshotOf">
        <rdfs:label>isSnapshotOf</rdfs:label>
        <rdfs:comment>Inverse of roevo:hasSnapshot. It associates an roevo:SnapshotRO with the roevo:LiveRO from which it was created</rdfs:comment>
    </owl:ObjectProperty>
    


    <!-- http://purl.org/wf4ever/roevo#relatedResource -->

    <owl:ObjectProperty rdf:about="&roevo;relatedResource">
        <rdfs:label>relatedResource</rdfs:label>
        <rdfs:comment>Associates a change (roevo:Change) to the resource (roevo:VersionableResource) affected by this change</rdfs:comment>
        <rdfs:domain rdf:resource="&roevo;Change"/>
        <rdfs:range rdf:resource="&roevo;VersionableResource"/>
        <rdfs:subPropertyOf rdf:resource="&prov;used"/>
    </owl:ObjectProperty>
    


    <!-- http://purl.org/wf4ever/roevo#toVersion -->

    <owl:ObjectProperty rdf:about="&roevo;toVersion">
        <rdfs:label>toVersion</rdfs:label>
        <rdfs:comment>Associates the set of changes (roevo:ChangeSpecification) that generated the pointed version of the resource (roevo:VersionableResource)</rdfs:comment>
        <rdfs:domain rdf:resource="&roevo;ChangeSpecification"/>
        <rdfs:range rdf:resource="&roevo;VersionableResource"/>
        <rdfs:subPropertyOf rdf:resource="&prov;generated"/>
    </owl:ObjectProperty>
    


    <!-- http://purl.org/wf4ever/roevo#wasArchivedBy -->

    <owl:ObjectProperty rdf:about="&roevo;wasArchivedBy">
        <rdfs:label>wasArchivedBy</rdfs:label>
        <rdfs:comment>Indicates the prov:Agent responsible for creating the associated roevo:ArchivedRO</rdfs:comment>
        <rdfs:domain rdf:resource="&roevo;ArchivedRO"/>
        <rdfs:range rdf:resource="&prov;Agent"/>
        <rdfs:subPropertyOf rdf:resource="&prov;wasAttributedTo"/>
    </owl:ObjectProperty>
    


    <!-- http://purl.org/wf4ever/roevo#wasChangedBy -->

    <owl:ObjectProperty rdf:about="&roevo;wasChangedBy">
        <rdfs:label>wasChangedBy</rdfs:label>
        <rdfs:comment>Associates a version of the resource (roevo:VersionableResource) to the set of changes (roevo:ChangeSpecification) that generated it</rdfs:comment>
        <rdfs:range rdf:resource="&roevo;ChangeSpecification"/>
        <rdfs:domain rdf:resource="&roevo;VersionableResource"/>
        <rdfs:subPropertyOf rdf:resource="&prov;wasGeneratedBy"/>
    </owl:ObjectProperty>
    


    <!-- http://purl.org/wf4ever/roevo#wasSnapshotedBy -->

    <owl:ObjectProperty rdf:about="&roevo;wasSnapshotedBy">
        <rdfs:label>wasSnapshotedBy</rdfs:label>
        <rdfs:comment>Indicates the prov:Agent responsible for creating the associated roevo:SnapshotRO</rdfs:comment>
        <rdfs:domain rdf:resource="&roevo;SnapshotRO"/>
        <rdfs:range rdf:resource="&prov;Agent"/>
        <rdfs:subPropertyOf rdf:resource="&prov;wasAttributedTo"/>
    </owl:ObjectProperty>
    


    <!-- http://www.w3.org/ns/prov#generated -->

    <owl:ObjectProperty rdf:about="&prov;generated"/>
    


    <!-- http://www.w3.org/ns/prov#hadOriginalSource -->

    <owl:ObjectProperty rdf:about="&prov;hadOriginalSource">
        <rdfs:range rdf:resource="&prov;Entity"/>
        <rdfs:domain rdf:resource="&prov;Entity"/>
        <rdfs:subPropertyOf rdf:resource="&prov;wasDerivedFrom"/>
    </owl:ObjectProperty>
    


    <!-- http://www.w3.org/ns/prov#used -->

    <owl:ObjectProperty rdf:about="&prov;used"/>
    


    <!-- http://www.w3.org/ns/prov#wasAssociatedWith -->

    <owl:ObjectProperty rdf:about="&prov;wasAssociatedWith">
        <rdfs:domain rdf:resource="&prov;Activity"/>
        <rdfs:range rdf:resource="&prov;Agent"/>
    </owl:ObjectProperty>
    
    
    
    <!-- http://www.w3.org/ns/prov#wasAttributedTo -->

    <owl:ObjectProperty rdf:about="&prov;wasAttributedTo"/>
    


    <!-- http://www.w3.org/ns/prov#wasDerivedFrom -->

    <owl:ObjectProperty rdf:about="&prov;wasDerivedFrom">
        <rdf:type rdf:resource="&owl;AsymmetricProperty"/>
        <rdf:type rdf:resource="&owl;IrreflexiveProperty"/>
        <rdfs:range rdf:resource="&prov;Entity"/>
        <rdfs:domain rdf:resource="&prov;Entity"/>
    </owl:ObjectProperty>
    


    <!-- http://www.w3.org/ns/prov#wasGeneratedBy -->

    <owl:ObjectProperty rdf:about="&prov;wasGeneratedBy"/>
    


    <!-- http://www.w3.org/ns/prov#wasQuotedFrom -->

    <owl:ObjectProperty rdf:about="&prov;wasQuotedFrom">
        <rdfs:domain rdf:resource="&prov;Entity"/>
        <rdfs:range rdf:resource="&prov;Entity"/>
        <rdfs:subPropertyOf rdf:resource="&prov;wasDerivedFrom"/>
    </owl:ObjectProperty>
    


    <!-- http://www.w3.org/ns/prov#wasRevisionOf -->

    <owl:ObjectProperty rdf:about="&prov;wasRevisionOf">
        <rdfs:range rdf:resource="&prov;Entity"/>
        <rdfs:domain rdf:resource="&prov;Entity"/>
        <rdfs:subPropertyOf rdf:resource="&prov;wasDerivedFrom"/>
    </owl:ObjectProperty>
    


    <!-- 
    ///////////////////////////////////////////////////////////////////////////////////////
    //
    // Data properties
    //
    ///////////////////////////////////////////////////////////////////////////////////////
     -->

    


    <!-- http://purl.org/dc/terms/identifier -->

    <owl:DatatypeProperty rdf:about="&dcterms;identifier"/>
    


    <!-- http://purl.org/wf4ever/roevo#archivedAtTime -->

    <owl:DatatypeProperty rdf:about="&roevo;archivedAtTime">
        <rdfs:label>archivedAtTime</rdfs:label>
        <rdfs:comment>The time at which an roevo:ArchiveRO was completely created and is available for use</rdfs:comment>
        <rdfs:domain rdf:resource="&roevo;ArchivedRO"/>
        <rdfs:range rdf:resource="&xsd;dateTime"/>
        <rdfs:subPropertyOf rdf:resource="&prov;generatedAtTime"/>
    </owl:DatatypeProperty>
    


    <!-- http://purl.org/wf4ever/roevo#snapshotedAtTime -->

    <owl:DatatypeProperty rdf:about="&roevo;snapshotedAtTime">
        <rdfs:label>snapshotedAtTime</rdfs:label>
        <rdfs:comment>The time at which an roevo:SnapshotRO was completely created and is available for use</rdfs:comment>
        <rdfs:domain rdf:resource="&roevo;SnapshotRO"/>
        <rdfs:range rdf:resource="&xsd;dateTime"/>
        <rdfs:subPropertyOf rdf:resource="&prov;generatedAtTime"/>
    </owl:DatatypeProperty>
    


    <!-- http://www.w3.org/ns/prov#endedAtTime -->

    <owl:DatatypeProperty rdf:about="&prov;endedAtTime">
        <rdf:type rdf:resource="&owl;FunctionalProperty"/>
        <rdfs:range rdf:resource="&xsd;dateTime"/>
        <rdfs:domain rdf:resource="&prov;Activity"/>
    </owl:DatatypeProperty>
    


    <!-- http://www.w3.org/ns/prov#generatedAtTime -->

    <owl:DatatypeProperty rdf:about="&prov;generatedAtTime"/>
    


    <!-- http://www.w3.org/ns/prov#startedAtTime -->

    <owl:DatatypeProperty rdf:about="&prov;startedAtTime">
        <rdf:type rdf:resource="&owl;FunctionalProperty"/>
        <rdfs:range rdf:resource="&xsd;dateTime"/>
        <rdfs:domain rdf:resource="&prov;Activity"/>
    </owl:DatatypeProperty>
    


    <!-- 
    ///////////////////////////////////////////////////////////////////////////////////////
    //
    // Classes
    //
    ///////////////////////////////////////////////////////////////////////////////////////
     -->

    


    <!-- http://purl.org/wf4ever/ro#AggregatedAnnotation -->

    <owl:Class rdf:about="&ro;AggregatedAnnotation">
        <rdfs:subClassOf>
            <owl:Restriction>
                <owl:onProperty rdf:resource="&ao;annotatesResource"/>
                <owl:someValuesFrom>
                    <owl:Class>
                        <owl:unionOf rdf:parseType="Collection">
                            <rdf:Description rdf:about="&roevo;Change"/>
                            <rdf:Description rdf:about="&roevo;ChangeSpecification"/>
                            <rdf:Description rdf:about="&roevo;VersionableResource"/>
                        </owl:unionOf>
                    </owl:Class>
                </owl:someValuesFrom>
            </owl:Restriction>
        </rdfs:subClassOf>
    </owl:Class>
    


    <!-- http://purl.org/wf4ever/ro#ResearchObject -->

    <owl:Class rdf:about="&ro;ResearchObject"/>
    


    <!-- http://purl.org/wf4ever/ro#Resource -->

    <owl:Class rdf:about="&ro;Resource"/>
    


    <!-- http://purl.org/wf4ever/roevo#Addition -->

    <owl:Class rdf:about="&roevo;Addition">
        <rdfs:label>Addition</rdfs:label>
        <rdfs:subClassOf rdf:resource="&roevo;Change"/>
        <rdfs:comment>A type of roevo:Change that changes the aggregation, content and/or structure of the Research Object by adding a resources or an annotation</rdfs:comment>
    </owl:Class>
    


    <!-- http://purl.org/wf4ever/roevo#ArchivedRO -->

    <owl:Class rdf:about="&roevo;ArchivedRO">
        <rdfs:label>ArchivedRO</rdfs:label>
        <rdfs:subClassOf rdf:resource="&ro;ResearchObject"/>
        <rdfs:subClassOf rdf:resource="&prov;Entity"/>
        <rdfs:comment>A subclass of ro:ResearchObject representing a type of Research Object in archival state. It is also a subclass of prov:Entity as this is a type of artifact with fixed aspects and for which we want to provide provenance. 

Archived ROs represent the final stage of a RO (release) where it has either reached a version that the author prescribes to be stable and meaningful and is appropriate for publication and long-term preservation, or it has been deprecated. They are therefore immutable, with no further changes or versions allowed</rdfs:comment>
    </owl:Class>
    


    <!-- http://purl.org/wf4ever/roevo#Change -->

    <owl:Class rdf:about="&roevo;Change">
        <rdfs:label>Change</rdfs:label>
        <rdfs:subClassOf rdf:resource="&prov;Activity"/>
        <rdfs:comment>A prov:Activity that changes the Research Object (RO) aggregation, content, structure, or the annotations about the RO or its aggregated resources.</rdfs:comment>
    </owl:Class>
    


    <!-- http://purl.org/wf4ever/roevo#ChangeSpecification -->

    <owl:Class rdf:about="&roevo;ChangeSpecification">
        <rdfs:label>ChangeSpecification</rdfs:label>
        <rdfs:subClassOf rdf:resource="&prov;Activity"/>
        <rdfs:comment>A collection of roevo:Changes activities representing the set of changes in a Research Object between two different versions</rdfs:comment>
    </owl:Class>
    


    <!-- http://purl.org/wf4ever/roevo#LiveRO -->

    <owl:Class rdf:about="&roevo;LiveRO">
        <rdfs:label>LiveRO</rdfs:label>
        <rdfs:subClassOf rdf:resource="&ro;ResearchObject"/>
        <rdfs:subClassOf rdf:resource="&prov;Entity"/>
        <rdfs:comment>A subclass of ro:ResearchObject representing a type of Research Object in live state. It is also a subclass of prov:Entity as this is a type of artifact with fixed aspects and for which we want to provide provenance. 

Live ROs  represent a work in progress. They are thus mutable as the content or state of their resources may change.</rdfs:comment>
    </owl:Class>
    


    <!-- http://purl.org/wf4ever/roevo#Modification -->

    <owl:Class rdf:about="&roevo;Modification">
        <rdfs:label>Modification</rdfs:label>
        <rdfs:subClassOf rdf:resource="&roevo;Change"/>
        <rdfs:comment>A type of roevo:Change that modifies the aggregation, content and/or structure of the Research Object by updating an aggregated resource content or an existing annotation</rdfs:comment>
    </owl:Class>
    


    <!-- http://purl.org/wf4ever/roevo#Removal -->

    <owl:Class rdf:about="&roevo;Removal">
        <rdfs:label>Removal</rdfs:label>
        <rdfs:subClassOf rdf:resource="&roevo;Change"/>
        <rdfs:comment>A type of roevo:Change that changes the aggregation, content and/or structure of the Research Object by removing a resources or an annotation</rdfs:comment>
    </owl:Class>
    


    <!-- http://purl.org/wf4ever/roevo#SnapshotRO -->

    <owl:Class rdf:about="&roevo;SnapshotRO">
        <rdfs:label>SnapshotRO</rdfs:label>
        <rdfs:subClassOf rdf:resource="&ro;ResearchObject"/>
        <rdfs:subClassOf rdf:resource="&prov;Entity"/>
        <rdfs:comment>A subclass of ro:ResearchObject representing a type of Research Object in snapshot state. It is also a subclass of prov:Entity as this is a type of artifact with fixed aspects and for which we want to provide provenance. 

Snapshot ROs are intended as a record of past activity, ready to be disseminated as a whole. They are immutable, and reflect the state of the Live RO at a certain time. </rdfs:comment>
    </owl:Class>
    


    <!-- http://purl.org/wf4ever/roevo#VersionableResource -->

    <owl:Class rdf:about="&roevo;VersionableResource">
        <rdfs:label>VersionableResource</rdfs:label>
        <owl:equivalentClass>
            <owl:Class>
                <owl:unionOf rdf:parseType="Collection">
                    <rdf:Description rdf:about="&ro;AggregatedAnnotation"/>
                    <rdf:Description rdf:about="&ro;Resource"/>
                    <rdf:Description rdf:about="&roevo;ArchivedRO"/>
                    <rdf:Description rdf:about="&roevo;SnapshotRO"/>
                </owl:unionOf>
            </owl:Class>
        </owl:equivalentClass>
        <rdfs:subClassOf rdf:resource="&prov;Entity"/>
        <rdfs:subClassOf>
            <owl:Restriction>
                <owl:onProperty rdf:resource="&dcterms;identifier"/>
                <owl:someValuesFrom rdf:resource="&rdfs;Literal"/>
            </owl:Restriction>
        </rdfs:subClassOf>
        <rdfs:comment>A prov:Entity representing a type of artifact that may be versioned and for which we want to track its different versions. This class is equivalent to the union of roevo:SnapshotRO, roevo:ArchivedRO, ro:Resource and ro:AggregatedAnnotation that are the artifacts for which we want to track their versions.</rdfs:comment>
    </owl:Class>
    


    <!-- http://www.w3.org/ns/prov#Activity -->

    <owl:Class rdf:about="&prov;Activity"/>
    


    <!-- http://www.w3.org/ns/prov#Agent -->

    <owl:Class rdf:about="&prov;Agent"/>
    


    <!-- http://www.w3.org/ns/prov#Entity -->

    <owl:Class rdf:about="&prov;Entity"/>
</rdf:RDF>



<!-- Generated by the OWL API (version 3.4.2) http://owlapi.sourceforge.net -->

