<?xml version="1.0"?>


<!DOCTYPE rdf:RDF [
    <!ENTITY terms "http://purl.org/dc/terms/" >
    <!ENTITY prov "http://www.w3.org/ns/prov#" >
    <!ENTITY wf-fd "http://purl.org/net/wf-fd#" >
    <!ENTITY p-plan "http://purl.org/net/p-plan#" >
    <!ENTITY vann "http://purl.org/vocab/vann/" >
    <!ENTITY owl "http://www.w3.org/2002/07/owl#" >
    <!ENTITY xsd "http://www.w3.org/2001/XMLSchema#" >
    <!ENTITY rdfs "http://www.w3.org/2000/01/rdf-schema#" >
    <!ENTITY rdf "http://www.w3.org/1999/02/22-rdf-syntax-ns#" >
]>


<rdf:RDF xmlns="http://purl.org/net/wfd#"
     xml:base="http://purl.org/net/wfd"
     xmlns:terms="http://purl.org/dc/terms/"
     xmlns:xsd="http://www.w3.org/2001/XMLSchema#"
     xmlns:vann="http://purl.org/vocab/vann/"
     xmlns:rdfs="http://www.w3.org/2000/01/rdf-schema#"
     xmlns:prov="http://www.w3.org/ns/prov#"
     xmlns:rdf="http://www.w3.org/1999/02/22-rdf-syntax-ns#"
     xmlns:p-plan="http://purl.org/net/p-plan#"
     xmlns:owl="http://www.w3.org/2002/07/owl#"
     xmlns:wf-fd="http://purl.org/net/wf-fd#">
    <owl:Ontology rdf:about="http://purl.org/net/wf-fd#">
        <rdfs:label xml:lang="en">Workflow Fragment Description Ontology</rdfs:label>
        <terms:created rdf:datatype="&xsd;date">2013-09-17</terms:created>
        <terms:creator rdf:datatype="&xsd;anyURI">http://delicias.dia.fi.upm.es/members/DGarijo/#me</terms:creator>
        <vann:preferredNamespaceUri>http://purl.org/net/wf-fd#</vann:preferredNamespaceUri>
        <vann:preferredNamespacePrefix>wffd</vann:preferredNamespacePrefix>
        <owl:versionInfo>1.0</owl:versionInfo>
        <terms:modified rdf:datatype="&xsd;date">2013-09-17</terms:modified>
        <terms:license>http://creativecommons.org/licenses/by-nc-sa/2.0/</terms:license>
        <rdfs:comment>P-Plan extension to represent workflow fragments and their relationships to workflow templates</rdfs:comment>
        <terms:description xml:lang="en">P-Plan extension to represent workflow fragments and their relationships to workflow templates</terms:description>
        <terms:title xml:lang="en">The Workflow Fragment Description ontology</terms:title>
        <owl:imports rdf:resource="http://purl.org/net/p-plan#"/>
    </owl:Ontology>
    


    <!-- 
    ///////////////////////////////////////////////////////////////////////////////////////
    //
    // Annotation properties
    //
    ///////////////////////////////////////////////////////////////////////////////////////
     -->

    


    <!-- 
    ///////////////////////////////////////////////////////////////////////////////////////
    //
    // Datatypes
    //
    ///////////////////////////////////////////////////////////////////////////////////////
     -->

    


    <!-- 
    ///////////////////////////////////////////////////////////////////////////////////////
    //
    // Object Properties
    //
    ///////////////////////////////////////////////////////////////////////////////////////
     -->

    


    <!-- http://purl.org/net/wf-fd#foundAs -->

    <owl:ObjectProperty rdf:about="&wf-fd;foundAs">
        <rdfs:label xml:lang="en">foundAs</rdfs:label>
        <rdfs:comment xml:lang="en">Property that links a Detected Result Workflow Fragment to a Bound Result Workflow Fragment. That is, this property links a workflow fragment found as a result of applying graph mining techniques to a collection of workflows to the correspondant fragment of the workflow itself.</rdfs:comment>
        <rdfs:isDefinedBy rdf:resource="http://purl.org/net/wf-fd#"/>
        <rdfs:domain rdf:resource="&wf-fd;DetectedResutlWorkflowFragment"/>
        <rdfs:range rdf:resource="&wf-fd;TiedResultWorkflowFragment"/>
    </owl:ObjectProperty>
    


    <!-- http://purl.org/net/wf-fd#overlapsWithWorkflowFragment -->

    <owl:ObjectProperty rdf:about="&wf-fd;overlapsWithWorkflowFragment">
        <rdf:type rdf:resource="&owl;SymmetricProperty"/>
        <rdfs:label xml:lang="en">overlapsWithWorkflowFragment</rdfs:label>
        <rdfs:comment xml:lang="en">Property that specifies which Detected Result Workflow Fragments overlap with each other. In this case an overlap means to be included partially as part of another fragment</rdfs:comment>
        <rdfs:isDefinedBy rdf:resource="http://purl.org/net/wf-fd#"/>
        <rdfs:domain rdf:resource="&wf-fd;DetectedResutlWorkflowFragment"/>
        <rdfs:range rdf:resource="&wf-fd;DetectedResutlWorkflowFragment"/>
    </owl:ObjectProperty>
    


    <!-- 
    ///////////////////////////////////////////////////////////////////////////////////////
    //
    // Classes
    //
    ///////////////////////////////////////////////////////////////////////////////////////
     -->

    


    <!-- http://purl.org/net/wf-fd#DetectedResutlWorkflowFragment -->

    <owl:Class rdf:about="&wf-fd;DetectedResutlWorkflowFragment">
        <rdfs:label xml:lang="en">Detected Result Workflow Fragment</rdfs:label>
        <rdfs:subClassOf rdf:resource="&wf-fd;WorkflowFragment"/>
        <rdfs:comment xml:lang="en">A Detected Result Workflow Fragment is a Workflow Fragment detected automatically by using graph matching tecnhiques over a workflow collection. This fragment is a result of the algortihms and it is composed of Detected Result Steps.</rdfs:comment>
        <rdfs:isDefinedBy rdf:resource="http://purl.org/net/wf-fd#"/>
    </owl:Class>
    


    <!-- http://purl.org/net/wf-fd#TiedResultWorkflowFragment -->

    <owl:Class rdf:about="&wf-fd;TiedResultWorkflowFragment">
        <rdfs:label xml:lang="en">Tied Result Workflow Fragment</rdfs:label>
        <rdfs:subClassOf rdf:resource="&wf-fd;WorkflowFragment"/>
        <rdfs:comment xml:lang="en">A Tied Workflow Result Fragment is a Workflow Fragment used as an auxiliary structure to point to Workflow Steps of a collection of workflows. </rdfs:comment>
        <rdfs:isDefinedBy rdf:resource="http://purl.org/net/wf-fd#"/>
    </owl:Class>
    


    <!-- http://purl.org/net/wf-fd#WorkflowFragment -->

    <owl:Class rdf:about="&wf-fd;WorkflowFragment">
        <rdfs:label xml:lang="en">Workflow Fragment</rdfs:label>
        <rdfs:subClassOf rdf:resource="&p-plan;Plan"/>
        <rdfs:comment xml:lang="en">A Workflow Fragment is a set of connected steps which belongs as part of a scientific workflow. A Workflow Fragment is a directed acyclic graph (DAG) and may have one or more Steps.

There are two types of Workflow Fragments: The Bound Result Workflow Fragments and the Detected Result Workflow Fragments. On one hand, the Detected Result Workflow Fragments are used to describe the results of the graph matching algorithms applied to a workflow collection. On the other hand, the Bound Workflow Result Fragments are auxiliary structures to point out the Steps of a Workflow belonging to a Detected Result Workflow Fragment .</rdfs:comment>
        <rdfs:isDefinedBy rdf:resource="http://purl.org/net/wf-fd#"/>
    </owl:Class>
    


    <!-- 
    ///////////////////////////////////////////////////////////////////////////////////////
    //
    // Individuals
    //
    ///////////////////////////////////////////////////////////////////////////////////////
     -->

    


    <!-- http://purl.org/net/wf-fd# -->

    <owl:Thing rdf:about="http://purl.org/net/wf-fd#">
        <rdf:type rdf:resource="&owl;NamedIndividual"/>
    </owl:Thing>
</rdf:RDF>



<!-- Generated by the OWL API (version 3.2.3.22702) http://owlapi.sourceforge.net -->

